code/poly1305/Hacl.Spec.Poly1305.Equiv.fst
@@ -7,360 +7,271 @@ open Lib.ByteSequence
 open Lib.IntVector
 
 module Loops = Lib.LoopCombinators
-module PLoops = Lib.Sequence.Lemmas
+module VecLemmas = Lib.Vec.Lemmas
+module SeqLemmas = Lib.Sequence.Lemmas
 module Lemmas = Hacl.Spec.Poly1305.Lemmas
 module S = Spec.Poly1305
 
 include Hacl.Spec.Poly1305.Vec
 
-#reset-options "--z3rlimit 100 --max_fuel 0 --max_ifuel 0"
+#set-options "--z3rlimit 50 --max_fuel 0 --max_ifuel 0"
 
-val poly_update_multi_lemma_load_acc1:
-    r:pfelem
-  -> text:bytes{size_block <= length text /\ length text % size_block = 0}
-  -> acc0:pfelem ->
-  Lemma
-   (let t0 = Seq.slice text 0 size_block in
-    let f = S.poly1305_update1 r size_block in
-    let repeat_bf_t0 = repeat_blocks_f size_block t0 f 1 in
-    normalize_n r (load_acc1 t0 acc0) == PLoops.repeat_w #pfelem 1 1 repeat_bf_t0 0 acc0)
+let block_v (w:lanes{w * size_block <= max_size_t}) = lbytes (w * size_block)
 
-let poly_update_multi_lemma_load_acc1 r text acc0 = ()
+///
+///  val load_acc_lemma: #w:lanes -> b:block_v w -> acc0:pfelem -> r:pfelem -> Lemma
+///   (normalize_n r (load_acc b acc0) == repeat_blocks_multi size_block b (S.poly1305_update1 r size_block) acc0)
+///
 
+val load_acc_lemma1: b:block_v 1 -> acc0:pfelem -> r:pfelem -> Lemma
+  (normalize_n r (load_acc #1 b acc0) ==
+   repeat_blocks_multi size_block b (S.poly1305_update1 r size_block) acc0)
 
-val poly_update_multi_lemma_load_acc2:
-    r:pfelem
-  -> text:bytes{2 * size_block <= length text /\ length text % (2 * size_block) = 0 /\ length text % size_block = 0}
-  -> acc0:pfelem ->
-  Lemma
-   (let t0 = Seq.slice text 0 (2 * size_block) in
-    let f = S.poly1305_update1 r size_block in
-    let repeat_bf_t0 = repeat_blocks_f size_block t0 f 2 in
-    normalize_n r (load_acc2 t0 acc0) == PLoops.repeat_w #pfelem 2 1 repeat_bf_t0 0 acc0)
-
-let poly_update_multi_lemma_load_acc2 r text acc0 =
-  let t0 = Seq.slice text 0 (2 * size_block) in
+let load_acc_lemma1 b acc0 r =
   let f = S.poly1305_update1 r size_block in
-  let repeat_bf_t0 = repeat_blocks_f size_block t0 f 2 in
-  assert (PLoops.repeat_w #pfelem 2 1 repeat_bf_t0 0 acc0 == repeat_bf_t0 1 (repeat_bf_t0 0 acc0));
+  let nb = size_block / size_block in
+  let repeat_f = repeat_blocks_f size_block b f nb in
 
-  let b0 = Seq.slice text 0 size_block in
-  let b1 = Seq.slice text size_block (2 * size_block) in
+  lemma_repeat_blocks_multi size_block b f acc0;
+  Loops.unfold_repeati nb repeat_f acc0 0;
+  Loops.eq_repeati0 nb repeat_f acc0
 
+
+val load_acc_lemma2: b:block_v 2 -> acc0:pfelem -> r:pfelem -> Lemma
+  (normalize_n r (load_acc b acc0) ==
+   repeat_blocks_multi size_block b (S.poly1305_update1 r size_block) acc0)
+
+let load_acc_lemma2 b acc0 r =
+  let b0 = Seq.slice b 0 size_block in
+  let b1 = Seq.slice b size_block (2 * size_block) in
   let c0 = pfadd (pow2 128) (nat_from_bytes_le b0) in
   let c1 = pfadd (pow2 128) (nat_from_bytes_le b1) in
-  assert (repeat_bf_t0 1 (repeat_bf_t0 0 acc0) == pfmul (pfadd (pfmul (pfadd acc0 c0) r) c1) r);
 
-  let acc1 = load_acc2 t0 acc0 in
-  let acc2 = normalize_n r acc1 in
-  assert (acc2 == pfadd (pfmul acc1.[0] (pfmul r r)) (pfmul acc1.[1] r));
-  assert (acc1.[0] == pfadd acc0 c0);
-  assert (acc1.[1] == pfadd 0 c1);
   FStar.Math.Lemmas.modulo_lemma c1 prime;
-  assert (acc1.[1] == c1);
-  assert (acc2 == pfadd (pfmul (pfadd acc0 c0) (pfmul r r)) (pfmul c1 r));
+
+  let f = S.poly1305_update1 r size_block in
+  let nb = (2 * size_block) / size_block in
+  let repeat_f = repeat_blocks_f size_block b f nb in
+
+  lemma_repeat_blocks_multi size_block b f acc0;
+  Loops.unfold_repeati nb repeat_f acc0 1;
+  Loops.unfold_repeati nb repeat_f acc0 0;
+  Loops.eq_repeati0 nb repeat_f acc0;
   Lemmas.poly_update_multi_lemma_load2_simplify acc0 r c0 c1
 
 
-val poly_update_multi_lemma_load_acc4:
-    r:pfelem
-  -> text:bytes{4 * size_block <= length text /\ length text % (4 * size_block) = 0 /\ length text % size_block = 0}
-  -> acc0:pfelem ->
-  Lemma
-   (let t0 = Seq.slice text 0 (4 * size_block) in
-    let f = S.poly1305_update1 r size_block in
-    let repeat_bf_t0 = repeat_blocks_f size_block t0 f 4 in
-    normalize_n r (load_acc4 t0 acc0) == PLoops.repeat_w #pfelem 4 1 repeat_bf_t0 0 acc0)
+val load_acc_lemma4: b:block_v 4 -> acc0:pfelem -> r:pfelem -> Lemma
+  (normalize_n r (load_acc b acc0) ==
+   repeat_blocks_multi size_block b (S.poly1305_update1 r size_block) acc0)
 
-let poly_update_multi_lemma_load_acc4 r text acc0 =
-  let t0 = Seq.slice text 0 (4 * size_block) in
-  let f = S.poly1305_update1 r size_block in
-  let repeat_bf_t0 = repeat_blocks_f size_block t0 f 4 in
-
-  let acc1 = PLoops.repeat_w #pfelem 4 1 repeat_bf_t0 0 acc0 in
-  assert (acc1 == repeat_bf_t0 3 (repeat_bf_t0 2 (repeat_bf_t0 1 (repeat_bf_t0 0 acc0))));
-
-  let b0 = Seq.slice text 0 size_block in
-  let b1 = Seq.slice text size_block (2 * size_block) in
-  let b2 = Seq.slice text (2 * size_block) (3 * size_block) in
-  let b3 = Seq.slice text (3 * size_block) (4 * size_block) in
+let load_acc_lemma4 b acc0 r =
+  let b0 = Seq.slice b 0 size_block in
+  let b1 = Seq.slice b size_block (2 * size_block) in
+  let b2 = Seq.slice b (2 * size_block) (3 * size_block) in
+  let b3 = Seq.slice b (3 * size_block) (4 * size_block) in
 
   let c0 = pfadd (pow2 128) (nat_from_bytes_le b0) in
   let c1 = pfadd (pow2 128) (nat_from_bytes_le b1) in
   let c2 = pfadd (pow2 128) (nat_from_bytes_le b2) in
   let c3 = pfadd (pow2 128) (nat_from_bytes_le b3) in
-  assert (acc1 == pfmul (pfadd (pfmul (pfadd (pfmul (pfadd (pfmul (pfadd acc0 c0) r) c1) r) c2) r) c3) r);
 
-  let acc2 = load_acc4 t0 acc0 in
-  let acc3 = normalize_4 r acc2 in
-  assert (acc2.[0] == pfadd acc0 c0);
   FStar.Math.Lemmas.modulo_lemma c1 prime;
   FStar.Math.Lemmas.modulo_lemma c2 prime;
   FStar.Math.Lemmas.modulo_lemma c3 prime;
-  assert (acc2.[1] == c1);
-  assert (acc2.[2] == c2);
-  assert (acc2.[3] == c3);
-  assert (acc3 ==
-    pfadd (pfadd (pfadd (pfmul (pfadd acc0 c0) (pfmul (pfmul r r) (pfmul r r)))
-      (pfmul c1 (pfmul (pfmul r r) r))) (pfmul c2 (pfmul r r))) (pfmul c3 r));
-  Lemmas.poly_update_multi_lemma_load4_simplify acc0 r c0 c1 c2 c3;
-  assert (acc1 == acc3)
 
-
-val poly_update_multi_lemma_load_acc:
-    #w:lanes
-  -> r:pfelem
-  -> text:bytes{w * size_block <= length text /\ length text % (w * size_block) = 0 /\ length text % size_block = 0}
-  -> acc0:pfelem ->
-  Lemma
-   (let t0 = Seq.slice text 0 (w * size_block) in
-    let f = S.poly1305_update1 r size_block in
-    let repeat_bf_t0 = repeat_blocks_f size_block t0 f w in
-    normalize_n r (load_acc #w t0 acc0) == PLoops.repeat_w #pfelem w 1 repeat_bf_t0 0 acc0)
-
-let poly_update_multi_lemma_load_acc #w r text acc0 =
-  match w with
-  | 1 -> poly_update_multi_lemma_load_acc1 r text acc0
-  | 2 -> poly_update_multi_lemma_load_acc2 r text acc0
-  | 4 -> poly_update_multi_lemma_load_acc4 r text acc0
-
-
-val poly_update_multi_lemma_loop1:
-    r:pfelem
-  -> text:bytes{size_block <= length text /\ length text % size_block = 0}
-  -> i:nat{i < (length text - size_block) / size_block}
-  -> acc_vec:elem 1 ->
-  Lemma
-   (let rw = compute_rw #1 r in
-    let len = length text in
-    let len1 = len - size_block in
-
-    let nb_vec = len1 / size_block in
-    let nb = len1 / size_block in
-    assert (nb == nb_vec);
-
-    let t1 = Seq.slice text size_block len in
-    let f = S.poly1305_update1 r size_block in
-    let f_vec = Vec.poly1305_update_nblocks rw in
-    let repeat_bf_vec = repeat_blocks_f size_block t1 f_vec nb_vec in
-    let repeat_bf_t1 = repeat_blocks_f size_block t1 f nb in
-    normalize_n r (repeat_bf_vec i acc_vec) == PLoops.repeat_w #pfelem 1 nb_vec repeat_bf_t1 i (normalize_n r acc_vec))
-
-let poly_update_multi_lemma_loop1 r text i acc_vec = ()
-
-
-val poly_update_multi_lemma_loop2:
-    r:pfelem
-  -> text:bytes{2 * size_block <= length text /\ length text % (2 * size_block) = 0 /\ length text % size_block = 0}
-  -> i:nat{i < (length text - 2 * size_block) / (2 * size_block)}
-  -> acc_vec:elem 2 ->
-  Lemma
-   (let rw = compute_rw #2 r in
-    let len = length text in
-    let len1 = len - 2 * size_block in
-
-    let nb_vec = len1 / (2 * size_block) in
-    let nb = len1 / size_block in
-    assert (nb == 2 * nb_vec);
-
-    let t1 = Seq.slice text (2 * size_block) len in
-    let f = S.poly1305_update1 r size_block in
-    let f_vec = Vec.poly1305_update_nblocks rw in
-    let repeat_bf_vec = repeat_blocks_f (2 * size_block) t1 f_vec nb_vec in
-    let repeat_bf_t1 = repeat_blocks_f size_block t1 f nb in
-    normalize_n r (repeat_bf_vec i acc_vec) == PLoops.repeat_w #pfelem 2 nb_vec repeat_bf_t1 i (normalize_n r acc_vec))
-
-let poly_update_multi_lemma_loop2 r text i acc_vec0 =
-  let rw = compute_rw #2 r in
-  let len = length text in
-  let len1 = len - 2 * size_block in
-
-  let nb_vec = len1 / (2 * size_block) in
-  let nb = len1 / size_block in
-  assert (nb == 2 * nb_vec);
-
-  let t1 = Seq.slice text (2 * size_block) len in
   let f = S.poly1305_update1 r size_block in
-  let f_vec = Vec.poly1305_update_nblocks rw in
-  let repeat_bf_vec = repeat_blocks_f (2 * size_block) t1 f_vec nb_vec in
-  let repeat_bf_t1 = repeat_blocks_f size_block t1 f nb in
+  let nb = (4 * size_block) / size_block in
+  let repeat_f = repeat_blocks_f size_block b f nb in
 
-  let acc1 = PLoops.repeat_w #pfelem 2 nb_vec repeat_bf_t1 i (normalize_n r acc_vec0) in
-  assert (acc1 == repeat_bf_t1 (2*i+1) (repeat_bf_t1 (2*i) (normalize_2 r acc_vec0)));
+  lemma_repeat_blocks_multi size_block b f acc0;
+  Loops.unfold_repeati nb repeat_f acc0 3;
+  Loops.unfold_repeati nb repeat_f acc0 2;
+  Loops.unfold_repeati nb repeat_f acc0 1;
+  Loops.unfold_repeati nb repeat_f acc0 0;
+  Loops.eq_repeati0 nb repeat_f acc0;
+  Lemmas.poly_update_multi_lemma_load4_simplify acc0 r c0 c1 c2 c3
 
-  let b0 = Seq.slice t1 (i * 32) (i * 32 + 16) in
-  let b1 = Seq.slice t1 (i * 32 + 16) (i * 32 + 32) in
+
+val load_acc_lemma: #w:lanes -> b:block_v w -> acc0:pfelem -> r:pfelem -> Lemma
+  (normalize_n r (load_acc b acc0) ==
+   repeat_blocks_multi size_block b (S.poly1305_update1 r size_block) acc0)
+
+let load_acc_lemma #w b acc0 r =
+  match w with
+  | 1 -> load_acc_lemma1 b acc0 r
+  | 2 -> load_acc_lemma2 b acc0 r
+  | 4 -> load_acc_lemma4 b acc0 r
+
+///
+///  val poly_update_nblocks_lemma: #w:lanes -> r:pfelem -> b:block_v w -> acc_v0:elem w -> Lemma
+///  (let rw = compute_rw r in
+///   normalize_n r (poly_update_nblocks #w rw b acc_v0) ==
+///   repeat_blocks_multi size_block b (poly_update1 r) (normalize_n r acc_v0))
+///
+
+val poly_update_nblocks_lemma1: r:pfelem -> b:block_v 1 -> acc_v0:elem 1 -> Lemma
+  (let rw = compute_rw #1 r in
+   normalize_n r (poly1305_update_nblocks rw b acc_v0) ==
+   repeat_blocks_multi size_block b (S.poly1305_update1 r size_block) (normalize_n r acc_v0))
+
+let poly_update_nblocks_lemma1 r b acc_v0 =
+  let acc0 = normalize_n r acc_v0 in
+  let f = S.poly1305_update1 r size_block in
+  let nb = size_block / size_block in
+  let repeat_f = repeat_blocks_f size_block b f nb in
+
+  lemma_repeat_blocks_multi size_block b f acc0;
+  Loops.unfold_repeati nb repeat_f acc0 0;
+  Loops.eq_repeati0 nb repeat_f acc0
+
+
+val poly_update_nblocks_lemma2: r:pfelem -> b:block_v 2 -> acc_v0:elem 2 -> Lemma
+  (let rw = compute_rw #2 r in
+   normalize_n r (poly1305_update_nblocks rw b acc_v0) ==
+   repeat_blocks_multi size_block b (S.poly1305_update1 r size_block) (normalize_n r acc_v0))
+
+let poly_update_nblocks_lemma2 r b acc_v0 =
+  let acc0 = normalize_n r acc_v0 in
+  let b0 = Seq.slice b 0 size_block in
+  let b1 = Seq.slice b size_block (2 * size_block) in
   let c0 = pfadd (pow2 128) (nat_from_bytes_le b0) in
   let c1 = pfadd (pow2 128) (nat_from_bytes_le b1) in
 
-  let acc_vec1 = repeat_bf_vec i acc_vec0 in
-  Lemmas.poly_update_repeat_blocks_multi_lemma2_simplify acc_vec0.[0] acc_vec0.[1] c0 c1 r;
-  assert (normalize_2 r acc_vec1 == PLoops.repeat_w #pfelem 2 nb_vec repeat_bf_t1 i (normalize_n r acc_vec0))
-
-
-#set-options "--z3rlimit 150"
-
-val poly_update_multi_lemma_loop4:
-    r:pfelem
-  -> text:bytes{4 * size_block <= length text /\ length text % (4 * size_block) = 0 /\ length text % size_block = 0}
-  -> i:nat{i < (length text - 4 * size_block) / (4 * size_block)}
-  -> acc_vec:elem 4 ->
-  Lemma
-   (let rw = compute_rw #4 r in
-    let len = length text in
-    let len1 = len - 4 * size_block in
-
-    let nb_vec = len1 / (4 * size_block) in
-    let nb = len1 / size_block in
-    assert (nb == 4 * nb_vec);
-
-    let t1 = Seq.slice text (4 * size_block) len in
-    let f = S.poly1305_update1 r size_block in
-    let f_vec = Vec.poly1305_update_nblocks rw in
-    let repeat_bf_vec = repeat_blocks_f (4 * size_block) t1 f_vec nb_vec in
-    let repeat_bf_t1 = repeat_blocks_f size_block t1 f nb in
-    normalize_n r (repeat_bf_vec i acc_vec) == PLoops.repeat_w #pfelem 4 nb_vec repeat_bf_t1 i (normalize_n r acc_vec))
-
-let poly_update_multi_lemma_loop4 r text i acc_vec0 =
-  let rw = compute_rw #4 r in
-  let len = length text in
-  let len1 = len - 4 * size_block in
-
-  let nb_vec = len1 / (4 * size_block) in
-  let nb = len1 / size_block in
-  assert (nb == 4 * nb_vec);
-
-  let t1 = Seq.slice text (4 * size_block) len in
   let f = S.poly1305_update1 r size_block in
-  let f_vec = Vec.poly1305_update_nblocks rw in
-  let repeat_bf_vec = repeat_blocks_f (4 * size_block) t1 f_vec nb_vec in
-  let repeat_bf_t1 = repeat_blocks_f size_block t1 f nb in
+  let nb = (2 * size_block) / size_block in
+  let repeat_f = repeat_blocks_f size_block b f nb in
 
-  let acc1 = PLoops.repeat_w #pfelem 4 nb_vec repeat_bf_t1 i (normalize_n r acc_vec0) in
-  assert (acc1 == repeat_bf_t1 (4*i+3) (repeat_bf_t1 (4*i+2)
-    (repeat_bf_t1 (4*i+1) (repeat_bf_t1 (4*i) (normalize_4 r acc_vec0)))));
+  lemma_repeat_blocks_multi size_block b f acc0;
+  Loops.unfold_repeati nb repeat_f acc0 1;
+  Loops.unfold_repeati nb repeat_f acc0 0;
+  Loops.eq_repeati0 nb repeat_f acc0;
+  Lemmas.poly_update_multi_lemma_load2_simplify acc0 r c0 c1;
+  Lemmas.poly_update_repeat_blocks_multi_lemma2_simplify acc_v0.[0] acc_v0.[1] c0 c1 r
 
-  let b0 = Seq.slice t1 (i * 64) (i * 64 + 16) in
-  let b1 = Seq.slice t1 (i * 64 + 16) (i * 64 + 32) in
-  let b2 = Seq.slice t1 (i * 64 + 32) (i * 64 + 48) in
-  let b3 = Seq.slice t1 (i * 64 + 48) (i * 64 + 64) in
+
+val poly_update_nblocks_lemma4: r:pfelem -> b:block_v 4 -> acc_v0:elem 4 -> Lemma
+  (let rw = compute_rw #4 r in
+   normalize_n r (poly1305_update_nblocks rw b acc_v0) ==
+   repeat_blocks_multi size_block b (S.poly1305_update1 r size_block) (normalize_n r acc_v0))
+
+let poly_update_nblocks_lemma4 r b acc_v0 =
+  let acc0 = normalize_n r acc_v0 in
+  let b0 = Seq.slice b 0 size_block in
+  let b1 = Seq.slice b size_block (2 * size_block) in
+  let b2 = Seq.slice b (2 * size_block) (3 * size_block) in
+  let b3 = Seq.slice b (3 * size_block) (4 * size_block) in
+
   let c0 = pfadd (pow2 128) (nat_from_bytes_le b0) in
   let c1 = pfadd (pow2 128) (nat_from_bytes_le b1) in
   let c2 = pfadd (pow2 128) (nat_from_bytes_le b2) in
   let c3 = pfadd (pow2 128) (nat_from_bytes_le b3) in
+
   let r2 = pfmul r r in
   let r4 = pfmul r2 r2 in
 
-  let acc_vec1 = repeat_bf_vec i acc_vec0 in
+  let f = S.poly1305_update1 r size_block in
+  let nb = (4 * size_block) / size_block in
+  let repeat_f = repeat_blocks_f size_block b f nb in
+
+  lemma_repeat_blocks_multi size_block b f acc0;
+  Loops.unfold_repeati nb repeat_f acc0 3;
+  Loops.unfold_repeati nb repeat_f acc0 2;
+  Loops.unfold_repeati nb repeat_f acc0 1;
+  Loops.unfold_repeati nb repeat_f acc0 0;
+  Loops.eq_repeati0 nb repeat_f acc0;
+
   Lemmas.poly_update_repeat_blocks_multi_lemma4_simplify
-    acc_vec0.[0] acc_vec0.[1] acc_vec0.[2] acc_vec0.[3] c0 c1 c2 c3 r r2 r4;
-  assert (normalize_n r acc_vec1 == PLoops.repeat_w #pfelem 4 nb_vec repeat_bf_t1 i (normalize_n r acc_vec0))
+    acc_v0.[0] acc_v0.[1] acc_v0.[2] acc_v0.[3] c0 c1 c2 c3 r r2 r4
 
 
-val poly_update_multi_lemma_loop:
-    #w:lanes
-  -> r:pfelem
-  -> text:bytes{w * size_block <= length text /\ length text % (w * size_block) = 0 /\ length text % size_block = 0}
-  -> i:nat{i < (length text - w * size_block) / (w * size_block)}
-  -> acc_vec:elem w ->
-  Lemma
-   (let rw = compute_rw #w r in
-    let len = length text in
-    let len1 = len - w * size_block in
+val poly_update_nblocks_lemma: #w:lanes -> r:pfelem -> b:block_v w -> acc_v0:elem w -> Lemma
+  (let rw = compute_rw #w r in
+   normalize_n r (poly1305_update_nblocks rw b acc_v0) ==
+   repeat_blocks_multi size_block b (S.poly1305_update1 r size_block) (normalize_n r acc_v0))
 
-    let nb_vec = len1 / (w * size_block) in
-    let nb = len1 / size_block in
-    assert (nb == w * nb_vec);
-
-    let t1 = Seq.slice text (w * size_block) len in
-    let f = S.poly1305_update1 r size_block in
-    let f_vec = Vec.poly1305_update_nblocks rw in
-    let repeat_bf_vec = repeat_blocks_f (w * size_block) t1 f_vec nb_vec in
-    let repeat_bf_t1 = repeat_blocks_f size_block t1 f nb in
-    normalize_n r (repeat_bf_vec i acc_vec) == PLoops.repeat_w #pfelem w nb_vec repeat_bf_t1 i (normalize_n r acc_vec))
-
-let poly_update_multi_lemma_loop #w r text i acc_vec =
+let poly_update_nblocks_lemma #w r b acc_v0 =
   match w with
-  | 1 -> poly_update_multi_lemma_loop1 r text i acc_vec
-  | 2 -> poly_update_multi_lemma_loop2 r text i acc_vec
-  | 4 -> poly_update_multi_lemma_loop4 r text i acc_vec
+  | 1 -> poly_update_nblocks_lemma1 r b acc_v0
+  | 2 -> poly_update_nblocks_lemma2 r b acc_v0
+  | 4 -> poly_update_nblocks_lemma4 r b acc_v0
+
+
+val repeat_blocks_multi_vec_equiv_pre_lemma: #w:lanes -> r:pfelem -> b:block_v w -> acc_v0:elem w -> Lemma
+  (let rw = compute_rw #w r in
+   let f = S.poly1305_update1 r size_block in
+   let f_v = poly1305_update_nblocks rw in
+   VecLemmas.repeat_blocks_multi_vec_equiv_pre w size_block f f_v (normalize_n r) b acc_v0)
+
+let repeat_blocks_multi_vec_equiv_pre_lemma #w r b acc_v0 =
+  poly_update_nblocks_lemma #w r b acc_v0
+
+
+val poly_update_multi_lemma_v:
+    #w:lanes
+  -> text:bytes{length text % (w * size_block) = 0 /\ length text % size_block = 0}
+  -> acc_v0:elem w
+  -> r:pfelem -> Lemma
+  (let rw = compute_rw #w r in
+   let f = S.poly1305_update1 r size_block in
+   let f_v = poly1305_update_nblocks rw in
+   normalize_n r (repeat_blocks_multi (w * size_block) text f_v acc_v0) ==
+   repeat_blocks_multi size_block text f (normalize_n r acc_v0))
+
+let poly_update_multi_lemma_v #w text acc_v0 r =
+  let rw = compute_rw #w r in
+  let f = S.poly1305_update1 r size_block in
+  let f_v = poly1305_update_nblocks rw in
+
+  Classical.forall_intro_2 (repeat_blocks_multi_vec_equiv_pre_lemma #w r);
+  VecLemmas.lemma_repeat_blocks_multi_vec w size_block text f f_v (normalize_n r) acc_v0
 
 
 val poly_update_multi_lemma:
     #w:lanes
   -> text:bytes{w * size_block <= length text /\ length text % (w * size_block) = 0 /\ length text % size_block = 0}
   -> acc0:pfelem
-  -> r:pfelem ->
-  Lemma
+  -> r:pfelem -> Lemma
   (poly1305_update_multi #w text acc0 r ==
-    repeat_blocks_multi #uint8 #pfelem size_block text (S.poly1305_update1 r size_block) acc0)
+   repeat_blocks_multi size_block text (S.poly1305_update1 r size_block) acc0)
 
 let poly_update_multi_lemma #w text acc0 r =
-  let rw = compute_rw #w r in
   let len = length text in
-  let len0 = w * size_block in
-  let len1 = len - len0 in
-  FStar.Math.Lemmas.modulo_addition_lemma len len0 (- 1);
-  assert (len % len0 == len1 % len0);
-
-  let t0 = Seq.slice text 0 len0 in
-  let t1 = Seq.slice text len0 len in
-
-  let acc1 = load_acc #w t0 acc0 in
-  let acc2 = repeat_blocks_multi #uint8 #(elem w) (w * size_block) t1 (poly1305_update_nblocks #w rw) acc1 in
-  let acc3 = normalize_n #w r acc2 in
-  assert (acc3 == poly1305_update_multi #w text acc0 r);
-
-  let nb_vec = len1 / (w * size_block) in
-  let nb = len1 / size_block in
-  assert (nb == w * nb_vec);
+  let blocksize_v = w * size_block in
+  let text0 = Seq.slice text 0 blocksize_v in
+  let text1 = Seq.slice text blocksize_v len in
+  FStar.Math.Lemmas.modulo_addition_lemma len blocksize_v (- 1);
+  assert (length text1 % (w * size_block) = 0 /\ length text1 % size_block = 0);
 
   let f = S.poly1305_update1 r size_block in
-  let f_vec = Vec.poly1305_update_nblocks rw in
+  let acc_v0 = load_acc #w text0 acc0 in
 
-  let repeat_bf_vec = repeat_blocks_f (w * size_block) t1 f_vec nb_vec in
-  let repeat_bf_t0 = repeat_blocks_f size_block t0 f w in
-  let repeat_bf_t1 = repeat_blocks_f size_block t1 f nb in
-
-  poly_update_multi_lemma_load_acc #w r text acc0;
-  //assert (normalize_n r (load_acc #w t0 acc0) == PLoops.repeat_w #pfelem w 1 repeat_bf_t0 0 acc0);
-  FStar.Classical.forall_intro_2 (poly_update_multi_lemma_loop #w r text);
-  //assert (forall (i:nat{i < nb_vec}) (acc_vec:elem w).
-    //  normalize_n r (repeat_bf_vec i acc_vec) == PLoops.repeat_w #pfelem w nb_vec repeat_bf_t1 i (normalize_n r acc_vec));
-
-  PLoops.lemma_repeat_blocks_multi_vec #uint8 #pfelem #(elem w)
-    w size_block text f f_vec (normalize_n r) (load_acc #w) acc0
+  let rp = poly1305_update_multi #w text acc0 r in
+  poly_update_multi_lemma_v #w text1 acc_v0 r;
+  load_acc_lemma #w text0 acc0 r;
+  SeqLemmas.repeat_blocks_multi_split size_block blocksize_v text f acc0
 
 
-val poly1305_update_vec_lemma:
-    #w:lanes
-  -> text:bytes
-  -> acc0:pfelem
-  -> r:pfelem ->
+val poly1305_update_vec_lemma: #w:lanes -> text:bytes -> acc0:pfelem -> r:pfelem ->
   Lemma (poly1305_update #w text acc0 r == S.poly1305_update text acc0 r)
 
 let poly1305_update_vec_lemma #w text acc0 r =
   let len = length text in
-  let sz_block = w * size_block in
-  let len0 = len / sz_block * sz_block in
-  FStar.Math.Lemmas.cancel_mul_mod (len / sz_block) sz_block;
-  assert (len0 % sz_block = 0);
+  let blocksize_v = w * size_block in
+  let len0 = len / blocksize_v * blocksize_v in
+  FStar.Math.Lemmas.cancel_mul_mod (len / blocksize_v) blocksize_v;
+  assert (len0 % blocksize_v = 0);
   assert (len0 % size_block = 0);
-  let t0 = Seq.slice text 0 len0 in
+
+  let text0 = Seq.slice text 0 len0 in
   let f = S.poly1305_update1 r size_block in
   let l = S.poly1305_update_last r in
 
-  if len0 > 0 then
-    begin
-    poly_update_multi_lemma #w t0 acc0 r;
-    PLoops.repeat_blocks_split #uint8 #pfelem size_block len0 text f l acc0
-    end
+  if len0 > 0 then begin
+    poly_update_multi_lemma #w text0 acc0 r;
+    SeqLemmas.repeat_blocks_split size_block len0 text f l acc0 end
 
 
-val poly1305_vec_lemma:
-    #w:lanes
-  -> msg:bytes
-  -> k:S.key ->
+val poly1305_vec_lemma: #w:lanes -> msg:bytes -> k:S.key ->
   Lemma (poly1305_mac #w msg k == S.poly1305_mac msg k)
 
 let poly1305_vec_lemma #w msg k =
